Hoare.v: support pre/post conditions on disk+memory

src/Hoare.v
@@ -4,105 +4,85 @@ Require Import Pred PredCrash.
 Require Import List.
 Require Import Morphisms.
 Require Import Word.
+Require Import Arith.
 
 Set Implicit Arguments.
 
 
 (** ** Hoare logic *)
 
-Definition donecond (T: Type) := T -> @mem addr (@weq addrlen) valuset -> Prop.
+Definition donecond (T: Type) := T -> @mem addr (@weq addrlen) valuset -> @mem nat eq_nat_dec mobj -> Prop.
 
-Definition corr2 (T: Type) (pre: donecond T -> pred -> pred) (p: prog T) :=
-  forall done crash m out, pre done crash m
-  -> exec m p out
-  -> (exists m' v, out = Finished m' v /\ done v m') \/
-     (exists m', out = Crashed T m' /\ crash m').
+Definition corr2 (T: Type) (pre: donecond T -> pred -> @mem _ (@weq addrlen) valuset -> @mem _ eq_nat_dec mobj -> Prop) (p: prog T) :=
+  forall done crash d m out, pre done crash d m
+  -> exec d m p out
+  -> (exists d' m' v, out = Finished d' m' v /\ done v d' m') \/
+     (exists d', out = Crashed T d' /\ crash d').
 
-Notation "{{ pre }} p" := (corr2 pre%pred p)
+Notation "{{ pre }} p" := (corr2 pre p)
   (at level 0, p at level 60).
 
 
-Definition corr3 (TF TR: Type) (pre: donecond TF -> donecond TR -> pred)
+Definition corr3 (TF TR: Type) (pre: donecond TF -> donecond TR -> @mem _ (@weq addrlen) valuset -> @mem _ eq_nat_dec mobj -> Prop)
                  (p1: prog TF) (p2: prog TR) :=
-  forall done crashdone m out, pre done crashdone m
-  -> exec_recover m p1 p2 out
-  -> (exists m' v, out = RFinished TR m' v /\ done v m') \/
-     (exists m' v, out = RRecovered TF m' v /\ crashdone v m').
+  forall done crashdone d m out, pre done crashdone d m
+  -> exec_recover d m p1 p2 out
+  -> (exists d' m' v, out = RFinished TR d' m' v /\ done v d' m') \/
+     (exists d' m' v, out = RRecovered TF d' m' v /\ crashdone v d' m').
 
-Notation "{{ pre }} p1 >> p2" := (corr3 pre%pred p1 p2)
+Notation "{{ pre }} p1 >> p2" := (corr3 pre p1 p2)
   (at level 0, p1 at level 60, p2 at level 60).
 
 Notation "'RET' : r post" :=
-  (fun F =>
-    (fun r => (F * post)%pred)
-  )%pred
+  (fun r => post)
   (at level 0, post at level 90, r at level 0, only parsing).
 
 Notation "'RET' : ^( ra , .. , rb ) post" :=
-  (fun F =>
-    (pair_args_helper (fun ra => ..
-      (pair_args_helper (fun rb (_:unit) => (F * post)%pred))
-    ..))
-  )%pred
+  (pair_args_helper (fun ra => ..
+    (pair_args_helper (fun rb (_:unit) => post))
+  ..))
   (at level 0, post at level 90, ra closed binder, rb closed binder, only parsing).
 
-Notation "{< e1 .. e2 , 'PRE' pre 'POST' post 'CRASH' crash >} p1" :=
+Notation "{< D M || e1 .. e2 , 'PRE' pre 'POST' post 'CRASH' crash >} p1" :=
   (forall T (rx: _ -> prog T), corr2
-   (fun done_ crash_ =>
+   (fun done_ crash_ disk_ mem_ =>
     (exis (fun e1 => .. (exis (fun e2 =>
-     exists F_,
-     F_ * pre *
-     [[ forall r_,
-        {{ fun done'_ crash'_ =>
-           post F_ r_ *
-           [[ done'_ = done_ ]] * [[ crash'_ = crash_ ]]
-        }} rx r_ ]] *
-     [[ (F_ * crash)%pred =p=> crash_ ]]
+     (fun D M => pre) disk_ mem_ /\
+     ( forall r_,
+       {{ fun done'_ crash'_ disk'_ mem'_ =>
+          (fun D M => post) disk'_ mem'_ r_ /\
+          done'_ = done_ /\
+          crash'_ = crash_
+       }} rx r_ ) /\
+     (fun D => crash) =p=> (fun D => crash_)
      )) .. ))
    )%pred
    (p1 rx)%pred)
   (at level 0, p1 at level 60, e1 binder, e2 binder).
 
-(**
- * The {!< .. >!} notation is the same as above, except it lacks a frame
- * predicate.  This is useful for bootstrapping-style programs.
- *)
-Notation "{!< e1 .. e2 , 'PRE' pre 'POST' post 'CRASH' crash >!} p1" :=
-  (forall T (rx: _ -> prog T), corr2
-   (fun done_ crash_ =>
-    (exis (fun e1 => .. (exis (fun e2 =>
-     pre *
-     [[ forall r_,
-        {{ fun done'_ crash'_ =>
-           post emp r_ *
-           [[ done'_ = done_ ]] * [[ crash'_ = crash_ ]]
-        }} rx r_ ]] *
-     [[ crash =p=> crash_ ]]
-     )) .. ))
-   )%pred
-   (p1 rx)%pred)
-  (at level 0, p1 at level 60, e1 binder, e2 binder).
 
 Definition forall_helper T (p : T -> Prop) :=
   forall v, p v.
 
-Notation "{<< e1 .. e2 , 'PRE' pre 'POST' post 'REC' crash >>} p1 >> p2" :=
+Notation "{<< D M || e1 .. e2 , 'PRE' pre 'POST' post 'REC' crash >>} p1 >> p2" :=
   (forall_helper (fun e1 => .. (forall_helper (fun e2 =>
    exists idemcrash,
    forall TF TR (rxOK: _ -> prog TF) (rxREC: _ -> prog TR),
    corr3
-   (fun done_ crashdone_ =>
-     exists F_,
-     F_ * pre *
-     [[ crash_xform F_ =p=> F_ ]] *
-     [[ forall r_,
-        {{ fun done'_ crash'_ => post F_ r_ *
-                                 [[ done'_ = done_ ]] * [[ crash'_ =p=> F_ * idemcrash ]]
-        }} rxOK r_ ]] *
-     [[ forall r_,
-        {{ fun done'_ crash'_ => crash F_ r_ *
-                                 [[ done'_ = crashdone_ ]] * [[ crash'_ =p=> F_ * idemcrash ]]
-        }} rxREC r_ ]]
+   (fun done_ crashdone_ disk_ mem_ =>
+     (fun D M => pre) disk_ mem_ /\
+     ( forall r_,
+       {{ fun done'_ crash'_ disk'_ mem'_ =>
+          (fun D M => post) disk'_ mem'_ r_ /\
+          done'_ = done_ /\
+          crash'_ =p=> idemcrash
+       }} rxOK r_ ) /\
+     ( forall r_,
+       {{ fun done'_ crash'_ disk'_ mem'_ =>
+          (fun D => crash) disk'_ r_ /\
+          done'_ = crashdone_ /\
+          crash'_ =p=> idemcrash
+       }} rxREC r_ )
    )%pred
    (p1 rxOK)%pred
    (p2 rxREC)%pred)) .. ))
@@ -113,23 +93,25 @@ Inductive corr3_result {A B : Type} :=
   | Complete : A -> corr3_result
   | Recover : B -> corr3_result.
 
-Notation "{<<< e1 .. e2 , 'PRE' pre 'POST' post >>>} p1 >> p2" :=
+Notation "{<<< D M || e1 .. e2 , 'PRE' pre 'POST' post >>>} p1 >> p2" :=
   (forall_helper (fun e1 => .. (forall_helper (fun e2 =>
    exists idemcrash,
    forall TF TR (rxOK: _ -> prog TF) (rxREC: _ -> prog TR),
    corr3
-   (fun done_ crashdone_ =>
-     exists F_,
-     F_ * pre *
-     [[ crash_xform F_ =p=> F_ ]] *
-     [[ forall r_,
-        {{ fun done'_ crash'_ => post F_ (Complete r_) *
-                                 [[ done'_ = done_ ]] * [[ crash'_ =p=> F_ * idemcrash ]]
-        }} rxOK r_ ]] *
-     [[ forall r_,
-        {{ fun done'_ crash'_ => post F_ (Recover r_) *
-                                 [[ done'_ = crashdone_ ]] * [[ crash'_ =p=> F_ * idemcrash ]]
-        }} rxREC r_ ]]
+   (fun done_ crashdone_ disk_ mem_ =>
+     (fun D M => pre) disk_ mem_ /\
+     ( forall r_,
+       {{ fun done'_ crash'_ disk'_ mem'_ =>
+          (fun D M => post) disk'_ mem'_ (Complete r_) /\
+          done'_ = done_ /\
+          crash'_ =p=> idemcrash
+       }} rxOK r_ ) /\
+     ( forall r_,
+       {{ fun done'_ crash'_ disk'_ mem'_ =>
+          (fun D M => post) disk'_ mem'_ (Recover r_) /\
+          done'_ = crashdone_ /\
+          crash'_ =p=> idemcrash
+       }} rxREC r_ )
    )%pred
    (p1 rxOK)%pred
    (p2 rxREC)%pred)) .. ))
@@ -138,139 +120,118 @@ Notation "{<<< e1 .. e2 , 'PRE' pre 'POST' post >>>} p1 >> p2" :=
 
 
 Theorem pimpl_ok2:
-  forall T pre pre' (pr: prog T),
+  forall T (pre pre' : _ -> _ -> _ -> _ -> Prop) (pr: prog T),
   {{pre'}} pr ->
-  (forall done crash, pre done crash =p=> pre' done crash) ->
+  (forall done crash d m, pre done crash d m -> pre' done crash d m) ->
   {{pre}} pr.
 Proof.
-  unfold corr2; intros.
-  eapply H; eauto.
-  eapply H0.
-  eauto.
+  unfold corr2; eauto.
 Qed.
 
 Theorem pimpl_ok3:
-  forall TF TR pre pre' (p: prog TF) (r: prog TR),
+  forall TF TR (pre pre' : _ -> _ -> _ -> _ -> Prop) (p: prog TF) (r: prog TR),
   {{pre'}} p >> r ->
-  (forall done crashdone, pre done crashdone =p=> pre' done crashdone) ->
+  (forall done crashdone d m, pre done crashdone d m -> pre' done crashdone d m) ->
   {{pre}} p >> r.
 Proof.
-  unfold corr3; intros.
-  eapply H; eauto.
-  eapply H0.
-  eauto.
+  unfold corr3; eauto.
 Qed.
 
 Theorem pimpl_ok2_cont :
-  forall T pre pre' A (k : A -> prog T) x y,
+  forall T (pre pre' : _ -> _ -> _ -> _ -> Prop) A (k : A -> prog T) x y,
   {{pre'}} k y ->
-  (forall done crash, pre done crash =p=> pre' done crash) ->
-  (forall done crash, pre done crash =p=> exists F, F * [[x = y]]) ->
+  (forall done crash d m, pre done crash d m -> pre' done crash d m) ->
+  (forall done crash d m, pre done crash d m -> x = y) ->
   {{pre}} k x.
 Proof.
-  unfold corr2, pimpl; intros.
+  unfold corr2; intros.
   edestruct H1; eauto.
-  eapply sep_star_lift_l in H4; [|instantiate (1:=([x=y])%pred)].
-  unfold lift in *; subst; eauto.
-  firstorder.
 Qed.
 
 Theorem pimpl_ok3_cont :
-  forall TF TR pre pre' A (k : A -> prog TF) x y (r: prog TR),
+  forall TF TR (pre pre' : _ -> _ -> _ -> _ -> Prop) A (k : A -> prog TF) x y (r: prog TR),
   {{pre'}} k y >> r ->
-  (forall done crashdone, pre done crashdone =p=> pre' done crashdone) ->
-  (forall done crashdone, pre done crashdone =p=> exists F, F * [[x = y]]) ->
+  (forall done crashdone d m, pre done crashdone d m -> pre' done crashdone d m) ->
+  (forall done crashdone d m, pre done crashdone d m -> x = y) ->
   {{pre}} k x >> r.
 Proof.
-  unfold corr3, pimpl; intros.
+  unfold corr3; intros.
   edestruct H1; eauto.
-  eapply sep_star_lift_l in H4; [|instantiate (1:=([x=y])%pred)].
-  unfold lift in *; subst; eauto.
-  firstorder.
 Qed.
 
 Theorem pimpl_pre2:
-  forall T pre pre' (pr: prog T),
-  (forall done crash, pre done crash =p=> [{{pre' done crash}} pr])
-  -> (forall done crash, pre done crash =p=> pre' done crash done crash)
+  forall T (pre : _ -> _ -> _ -> _ -> Prop) pre' (pr: prog T),
+  (forall done crash d m, pre done crash d m -> {{pre' done crash}} pr)
+  -> (forall done crash d m, pre done crash d m -> pre' done crash done crash d m)
   -> {{pre}} pr.
 Proof.
-  unfold corr2; intros.
-  eapply H; eauto.
-  eapply H0.
-  eauto.
+  unfold corr2; eauto.
 Qed.
 
 Theorem pimpl_pre3:
-  forall TF TR pre pre' (p: prog TF) (r: prog TR),
-  (forall done crashdone, pre done crashdone =p=> [{{pre' done crashdone}} p >> r])
-  -> (forall done crashdone, pre done crashdone =p=> pre' done crashdone done crashdone)
+  forall TF TR (pre : _ -> _ -> _ -> _ -> Prop) pre' (p: prog TF) (r: prog TR),
+  (forall done crashdone d m, pre done crashdone d m -> {{pre' done crashdone}} p >> r)
+  -> (forall done crashdone d m, pre done crashdone d m -> pre' done crashdone done crashdone d m)
   -> {{pre}} p >> r.
 Proof.
-  unfold corr3; intros.
-  eapply H; eauto.
-  eapply H0.
-  eauto.
+  unfold corr3; eauto.
 Qed.
 
 Theorem pre_false2:
-  forall T pre (p: prog T),
-  (forall done crash, pre done crash =p=> [False])
+  forall T (pre : _ -> _ -> _ -> _ -> Prop) (p: prog T),
+  (forall done crash d m, pre done crash d m -> False)
   -> {{ pre }} p.
 Proof.
-  unfold corr2; intros; exfalso.
-  eapply H; eauto.
+  unfold corr2; intros; exfalso; eauto.
 Qed.
 
 Theorem pre_false3:
-  forall TF TR pre (p: prog TF) (r: prog TR),
-  (forall done crashdone, pre done crashdone =p=> [False])
+  forall TF TR (pre : _ -> _ -> _ -> _ -> Prop) (p: prog TF) (r: prog TR),
+  (forall done crashdone d m, pre done crashdone d m -> False)
   -> {{ pre }} p >> r.
 Proof.
-  unfold corr3; intros; exfalso.
-  eapply H; eauto.
+  unfold corr3; intros; exfalso; eauto.
 Qed.
 
 
 Theorem corr2_exists:
   forall T R pre (p: prog R),
-  (forall (a:T), {{ fun done crash => pre done crash a }} p)
-  -> {{ fun done crash => exists a:T, pre done crash a }} p.
+  (forall (a:T), {{ fun done crash d m => pre done crash d m a }} p)
+  -> {{ fun done crash d m => exists a:T, pre done crash d m a }} p.
 Proof.
   unfold corr2; intros.
   destruct H0.
-  eapply H; eauto.
+  eauto.
 Qed.
 
 Theorem corr3_exists:
   forall T RF RR pre (p: prog RF) (r: prog RR),
-  (forall (a:T), {{ fun done crashdone => pre done crashdone a }} p >> r)
-  -> {{ fun done crashdone => exists a:T, pre done crashdone a }} p >> r.
+  (forall (a:T), {{ fun done crashdone d m => pre done crashdone d m a }} p >> r)
+  -> {{ fun done crashdone d m => exists a:T, pre done crashdone d m a }} p >> r.
 Proof.
   unfold corr3; intros.
   destruct H0.
-  eapply H; eauto.
+  eauto.
 Qed.
 
 Theorem corr2_forall: forall T R pre (p: prog R),
-  {{ fun done crash => exists a:T, pre done crash a }} p
-  -> forall (a:T), {{ fun done crash => pre done crash a }} p.
+  {{ fun done crash d m => exists a:T, pre done crash d m a }} p
+  -> forall (a:T), {{ fun done crash d m => pre done crash d m a }} p.
 Proof.
   unfold corr2; intros.
   eapply H; eauto.
-  exists a; eauto.
 Qed.
 
 Theorem corr3_forall: forall T RF RR pre (p: prog RF) (r: prog RR),
-  {{ fun done crashdone => exists a:T, pre done crashdone a }} p >> r
-  -> forall (a:T), {{ fun done crashdone => pre done crashdone a }} p >> r.
+  {{ fun done crashdone d m => exists a:T, pre done crashdone d m a }} p >> r
+  -> forall (a:T), {{ fun done crashdone d m => pre done crashdone d m a }} p >> r.
 Proof.
   unfold corr3; intros.
   eapply H; eauto.
-  exists a; eauto.
 Qed.
 
 
+(*
 Instance corr2_proper {T : Type} :
   Proper (pointwise_relation (donecond T) (pointwise_relation pred piff)
           ==> eq ==> iff) (@corr2 T).
@@ -286,3 +247,4 @@ Proof.
   intros a b Hab x y Hxy p q Hpq; subst.
   split; intros; eapply pimpl_ok3; try eassumption; apply Hab.
 Qed.
+*)
